Changing label-free language for lang. equiv

label-free/Semantics.v
@@ -1,155 +1,99 @@
-Require Export Syntax.
-Require Export Substitution.
+Require Import Syntax.
+Require Import Substitution.
 Require Import LibList.
 Require Import LibListSorted.
 Require Import LibRelation.
 
-(*
-(* Test standard permutations *)
-Require Import List.
-Require Import Sorting.Permutation.
-
-(* Notations & definitions *)
-Notation "l & x" := (l ++ (x::nil)) 
-  (at level 28, left associativity) : list_scope.
-Definition permut := (@Permutation (list ty)).
-
-Lemma PermutLastSame:
-forall G G' elem
-  (HT: permut (G & elem) (G' & elem)),
-  permut G G'.
-intros;
-apply Permutation_app_inv_r in HT.
-assumption.
-Qed.
-
-Lemma InConsNeq:
-forall A G (elem:A) elem',
-  elem<>elem' -> In elem (G&elem') -> In elem G.
-intros.
-apply in_app_or in H0.
-destruct H0.
-assumption.
-apply in_inv in H0. destruct H0.
-symmetry in H0; contradiction.
-apply in_nil in H0; contradiction.
-Qed.
-
-Lemma PermutationElementSplit_Neq:
-forall G G' H elem elem'
-  (HNeq: elem <> elem')
-  (HT: permut (G & elem ++ G') (H & elem')),
-  exists GH, exists GT, H = GH & elem ++ GT.
-intros.
-assert (exists G0, exists G1, H = G0 ++ elem::G1). 
-apply in_split.
-apply InConsNeq with (elem':=elem').
-assumption.
-apply Permutation_in with (l:=G & elem ++ G').
-assumption.
-apply in_or_app.
-left; apply in_or_app.
-right; apply in_eq.
-(* after assert *)
-destruct H0 as [GH]; destruct H0 as [GT];
-exists GH; exists GT.
-subst H;
-rewrite <- app_assoc.
-simpl; reflexivity.
-Qed.
-
-(* / *)
-*)
-
-Open Scope is5_scope.
+Open Scope label_free_is5_scope.
 
 Global Reserved Notation " G '|=' Gamma '|-' M ':::' A " (at level 70).
 
-Definition Context := list ty.
+Definition Context_LF := list ty_LF.
+Definition Background_LF := list Context_LF.
 
 (* Statics *)
-Inductive types: list Context -> Context -> te -> ty -> Prop :=
-| t_hyp: forall A G Gamma v_n
+Inductive types_LF: Background_LF -> Context_LF -> te_LF -> ty_LF -> Prop :=
+| t_hyp_LF: forall A G Gamma v_n
   (HT: nth_error Gamma v_n = Some A),
-  G |= Gamma |- (hyp v_n) ::: A
-| t_lam: forall A B G Gamma M 
+  G |= Gamma |- (hyp_LF v_n) ::: A
+| t_lam_LF: forall A B G Gamma M 
   (HT: G |= A::Gamma |- M ::: B),
-  G |= Gamma |- (lam A M) ::: A ---> B
-| t_appl: forall A B G Gamma M N
+  G |= Gamma |- (lam_LF A M) ::: A ---> B
+| t_appl_LF: forall A B G Gamma M N
   (HT1: G |= Gamma |- M ::: A ---> B)
   (HT2: G |= Gamma |- N ::: A),
-  G |= Gamma |- (appl M N) ::: B
-| t_box: forall A G Gamma M
+  G |= Gamma |- (appl_LF M N) ::: B
+| t_box_LF: forall A G Gamma M
   (HT: G & Gamma |= nil |- M ::: A),
-  G |= Gamma |- (box M) ::: [*] A
-| t_unbox: forall A G Gamma M
+  G |= Gamma |- (box_LF M) ::: [*] A
+| t_unbox_LF: forall A G Gamma M
   (HT: G |= Gamma |- M ::: [*] A),
-  G |= Gamma |- unbox M ::: A
-| t_unbox_fetch: forall A G Gamma Gamma' M
+  G |= Gamma |- unbox_LF M ::: A
+| t_unbox_fetch_LF: forall A G Gamma Gamma' M
   (HT: G & Gamma' |= Gamma |- M ::: [*] A),
-  forall G0, permut (G & Gamma) G0 -> G0 |= Gamma' |- unbox_fetch M ::: A
-| t_here: forall A G Gamma M
+  forall G0, permut (G & Gamma) G0 -> G0 |= Gamma' |- unbox_fetch_LF M ::: A
+| t_here_LF: forall A G Gamma M
   (HT: G |= Gamma |- M ::: A),
-  G |= Gamma |- here M ::: <*> A
-| t_get_here: forall A G Gamma Gamma' M
+  G |= Gamma |- here_LF M ::: <*> A
+| t_get_here_LF: forall A G Gamma Gamma' M
   (HT: G & Gamma' |= Gamma |- M ::: A),
-  forall G0, permut (G & Gamma) G0 -> G0 |= Gamma' |- get_here M ::: <*> A
-| t_letdia: forall A B G Gamma M N
+  forall G0, permut (G & Gamma) G0 -> G0 |= Gamma' |- get_here_LF M ::: <*> A
+| t_letdia_LF: forall A B G Gamma M N
   (HT1: G |= Gamma |- M ::: <*> A)
   (HT2: (A :: nil) :: G |= Gamma |- N ::: B),
-  G |= Gamma |- letdia M N ::: B 
-| t_letdia_get: forall A B G Gamma Gamma' M N
+  G |= Gamma |- letdia_LF M N ::: B 
+| t_letdia_get_LF: forall A B G Gamma Gamma' M N
   (HT1: G & Gamma' |= Gamma |- M ::: <*> A)
   (HT2: (A :: nil) :: G & Gamma |= Gamma' |- N ::: B),
-  forall G0, permut (G & Gamma) G0 -> G0 |= Gamma' |- letdia_get M N ::: B
-where " G '|=' Gamma '|-' M ':::' A " := (types G Gamma M A).
+  forall G0, permut (G & Gamma) G0 -> G0 |= Gamma' |- letdia_get_LF M N ::: B
+where " G '|=' Gamma '|-' M ':::' A " := (types_LF G Gamma M A) : label_free_is5_scope.
 
 (* Dynamics *)
 
-Inductive value: te -> Prop :=
-| val_lam: forall A M, value (lam A M)
-| val_box: forall M, value (box M)
-| val_here: forall M, value M -> value (here M)
-| val_get_here: forall M, value M -> value (get_here M)
+Inductive value_LF: te_LF -> Prop :=
+| val_lam_LF: forall A M, value_LF (lam_LF A M)
+| val_box_LF: forall M, value_LF (box_LF M)
+| val_here_LF: forall M, value_LF M -> value_LF (here_LF M)
+| val_get_here_LF: forall M, value_LF M -> value_LF (get_here_LF M)
 .
 
 Global Reserved Notation " M |-> N " (at level 70).
 
-Inductive step: te -> te -> Prop :=
-| red_appl_lam: forall M A N, appl (lam A M) N |-> [N//0] M
-| red_unbox_box: forall M, unbox (box M) |-> M
-| red_unbox_fetch_box: forall M, unbox_fetch (box M) |-> M
-| red_letdia_here: forall M N, letdia (here M) N |-> [M//0]N
-| red_letdia__get_here: forall M N, letdia (get_here M) N |-> [M//0]N
-| red_letdia_get__here: forall M N, letdia_get (here M) N |-> [M//0]N
-| red_letdia_get_get_here: forall M N, letdia_get (get_here M) N |-> [M//0]N
-| red_appl: forall M N M' (HT: M |-> M'), appl M N |-> appl M' N
-| red_unbox: forall M M' (HT: M |-> M'), unbox M |-> unbox M'
-| red_unbox_fetch: forall M M' (HT: M |-> M'), unbox_fetch M |-> unbox_fetch M'
-| red_dia_here: forall M M' (HT: M |-> M'), here M |-> here M'
-| red_dia_move: forall M M' (HT: M |-> M'), get_here M |-> get_here M'
-| red_letdia: forall M N M' (HT: M |-> M'), letdia M N |-> letdia M' N
-| red_letdia_move: forall M N M' (HT: M |-> M'), letdia_get M N |-> letdia_get M' N
-where " M |-> N " := (step M N ) : is5_scope.
-
+Inductive step_LF: te_LF -> te_LF -> Prop :=
+| red_appl_lam_LF: forall M A N, appl_LF (lam_LF A M) N |-> [N//0] M
+| red_unbox_box_LF: forall M, unbox_LF (box_LF M) |-> M
+| red_unbox_fetch_box_LF: forall M, unbox_fetch_LF (box_LF M) |-> M
+| red_letdia_here_LF: forall M N, letdia_LF (here_LF M) N |-> [M//0]N
+| red_letdia__get_here_LF: forall M N, letdia_LF (get_here_LF M) N |-> [M//0]N
+| red_letdia_get__here_LF: forall M N, letdia_get_LF (here_LF M) N |-> [M//0]N
+| red_letdia_get_get_here_LF: forall M N, letdia_get_LF (get_here_LF M) N |-> [M//0]N
+| red_appl_LF: forall M N M' (HT: M |-> M'), appl_LF M N |-> appl_LF M' N
+| red_unbox_LF: forall M M' (HT: M |-> M'), unbox_LF M |-> unbox_LF M'
+| red_unbox_fetch_LF: forall M M' (HT: M |-> M'), unbox_fetch_LF M |-> unbox_fetch_LF M'
+| red_dia_here_LF: forall M M' (HT: M |-> M'), here_LF M |-> here_LF M'
+| red_dia_move_LF: forall M M' (HT: M |-> M'), get_here_LF M |-> get_here_LF M'
+| red_letdia_LF: forall M N M' (HT: M |-> M'), letdia_LF M N |-> letdia_LF M' N
+| red_letdia_move_LF: forall M N M' (HT: M |-> M'), letdia_get_LF M N |-> letdia_get_LF M' N
+where " M |-> N " := (step_LF M N ) : label_free_is5_scope.
 
 Section Lemmas.
 
 Lemma eq_context_dec:
-forall Gamma Gamma': Context, {Gamma = Gamma'} + {Gamma <> Gamma'}.
+forall Gamma Gamma': Context_LF, {Gamma = Gamma'} + {Gamma <> Gamma'}.
   intros; decide equality; decide equality.
 Qed.
 
 (* TODO: this may be moved to a separate file *)
-
 (* Permutation *)
 
+(* TODO *)
 Lemma PermutLastSame:
 forall A G G' (elem:A)
   (HT: permut (G & elem) (G' & elem)),
   permut G G'.
 Admitted.
 
+(* TODO *)
 Lemma PermutationElementSplit_Neq:
 forall A G G' H (elem:A) (elem':A)
   (HNeq: elem <> elem')
@@ -157,17 +101,15 @@ forall A G G' H (elem:A) (elem':A)
   exists GH, exists GT, H = GH & elem ++ GT.
 Admitted.
 
-(* / Permutation *)
-
 (* TODO: not automated enough *)
 Lemma BackgroundSubsetImpl:
 forall G G' Gamma M A
   (HT: G |= Gamma |- M ::: A)
   (HSubst: exists GT, permut (G++GT) G'),
   G' |= Gamma |- M ::: A.
-intros.
-generalize dependent G'.
-induction HT; intros; eauto using types.
+intros;
+generalize dependent G';
+induction HT; intros; eauto using types_LF.
 (* box *)
 destruct HSubst as [GT];
 constructor;
@@ -175,26 +117,26 @@ apply IHHT;
 exists GT; permut_simpl; assumption.
 (* unbox_fetch *)
 destruct HSubst as [GT];
-apply t_unbox_fetch with (Gamma:=Gamma) (G:=G++GT).
+apply t_unbox_fetch_LF with (Gamma:=Gamma) (G:=G++GT).
 apply IHHT;
   exists GT; permut_simpl.
 apply permut_trans with (l2:= G0 ++ GT); 
 [ permut_simpl | ]; assumption.
 (* get_here *)
 destruct HSubst as [GT];
-apply t_get_here with (Gamma:=Gamma) (G:=G++GT).
+apply t_get_here_LF with (Gamma:=Gamma) (G:=G++GT).
 apply IHHT;
   exists GT; permut_simpl.
 apply permut_trans with (l2:= G0 ++ GT); 
 [ permut_simpl | ]; assumption.
 (* letdia *)
-apply t_letdia with (A:=A). 
+apply t_letdia_LF with (A:=A). 
 apply IHHT1; assumption.
 apply IHHT2; destruct HSubst as [GT];
 exists GT; permut_simpl; assumption.
 (* letdia_get *)
 destruct HSubst as [GT];
-apply t_letdia_get with (A:=A)(Gamma:=Gamma) (G:=G++GT).
+apply t_letdia_get_LF with (A:=A)(Gamma:=Gamma) (G:=G++GT).
 apply IHHT1;
   exists GT; permut_simpl.
 apply IHHT2;
@@ -220,10 +162,10 @@ forall G Gamma M A
     permut G (G' & Delta) ->
     G' & (Delta ++ Delta') |= Gamma |- M ::: A) /\ 
   (forall Gamma', G |= Gamma ++ Gamma' |- M ::: A).
-intros.
+intros;
 induction HT; split; intros.
 (* hyp *)
-eauto using types.
+eauto using types_LF.
 constructor; generalize dependent v_n;
 induction Gamma; destruct v_n; intros;
 simpl in HT; try discriminate; simpl;
@@ -250,19 +192,18 @@ constructor; apply IHHT; assumption.
 destruct (eq_context_dec Gamma Delta).
 (* = *)
 subst;
-apply t_unbox_fetch with (Gamma:=Delta++Delta') (G:=G).
+apply t_unbox_fetch_LF with (Gamma:=Delta++Delta') (G:=G).
   apply IHHT.
   apply permut_app_l;
-  apply PermutLastSame with (elem:=Delta); (* sad panda 8( *)
+  apply PermutLastSame with (elem:=Delta);
   apply permut_trans with (l2:=G0); assumption.
 (* <> *)
 assert (exists G0, exists G1, G' = G0 & Gamma ++ G1).
-  (* very sad panda 8( *)
   apply PermutationElementSplit_Neq with (G:=G) (G':=nil) (elem':=Delta).
     assumption.
     rew_app; apply permut_trans with (l2:=G0); assumption.
 destruct H1 as [GH]; destruct H1 as [GT]; subst G';
-apply t_unbox_fetch with (Gamma:=Gamma) (G:=GH ++ GT & (Delta ++ Delta')).
+apply t_unbox_fetch_LF with (Gamma:=Gamma) (G:=GH ++ GT & (Delta ++ Delta')).
 apply BackgroundSubsetImpl with (G:= (GH ++ GT & Gamma') & (Delta ++ Delta')).
   apply IHHT; permut_simpl;
   apply PermutLastSame with (elem := Gamma);
@@ -274,7 +215,7 @@ apply BackgroundSubsetImpl with (G:= (GH ++ GT & Gamma') & (Delta ++ Delta')).
   exists nil; permut_simpl.
 permut_simpl.
 (* unbox_fetch 2 *)
-apply t_unbox_fetch with (G:=G) (Gamma:=Gamma).
+apply t_unbox_fetch_LF with (G:=G) (Gamma:=Gamma).
   apply IHHT; permut_simpl.
   assumption.
 (* here *)
@@ -284,10 +225,10 @@ constructor; apply IHHT; assumption.
 destruct (eq_context_dec Gamma Delta).
 (* = *)
 subst;
-apply t_get_here with (Gamma:=Delta++Delta') (G:=G).
+apply t_get_here_LF with (Gamma:=Delta++Delta') (G:=G).
   apply IHHT.
   apply permut_app_l;
-  apply PermutLastSame with (elem:=Delta); (* sad panda 8( *)
+  apply PermutLastSame with (elem:=Delta);
   apply permut_trans with (l2:=G0); assumption.
 (* <> *)
 assert (exists G0, exists G1, G' = G0 & Gamma ++ G1).
@@ -295,7 +236,7 @@ assert (exists G0, exists G1, G' = G0 & Gamma ++ G1).
     assumption.
     rew_app; apply permut_trans with (l2:=G0); assumption.
 destruct H1 as [GH]; destruct H1 as [GT]; subst G';
-apply t_get_here with (Gamma:=Gamma) (G:=GH ++ GT & (Delta ++ Delta')).
+apply t_get_here_LF with (Gamma:=Gamma) (G:=GH ++ GT & (Delta ++ Delta')).
 apply BackgroundSubsetImpl with (G:= (GH ++ GT & Gamma') & (Delta ++ Delta')).
   apply IHHT; permut_simpl;
   apply PermutLastSame with (elem := Gamma);
@@ -307,23 +248,23 @@ apply BackgroundSubsetImpl with (G:= (GH ++ GT & Gamma') & (Delta ++ Delta')).
   exists nil; permut_simpl.
 permut_simpl.
 (* get_here 2 *)
-apply t_get_here with (G:=G) (Gamma:=Gamma).
+apply t_get_here_LF with (G:=G) (Gamma:=Gamma).
   apply IHHT; permut_simpl.
   assumption.
 (* letdia *)
-apply t_letdia with (A:=A).
+apply t_letdia_LF with (A:=A).
 apply IHHT1; assumption.
-apply IHHT2 with (G':=(A::nil)::G'). 
-permut_simpl.
+apply IHHT2 with (G':=(A::nil)::G');
+permut_simpl;
 assumption.
-apply t_letdia with (A:=A).
+apply t_letdia_LF with (A:=A).
 apply IHHT1; assumption.
 apply IHHT2. 
 (* letdia_get 1 *)
 destruct (eq_context_dec Gamma Delta).
 (* = *)
 subst;
-apply t_letdia_get with (A:=A)(Gamma:=Delta++Delta') (G:=G).
+apply t_letdia_get_LF with (A:=A)(Gamma:=Delta++Delta') (G:=G).
 apply IHHT1; assumption.
 apply BackgroundSubsetImpl with (G:=((A::nil) :: G) & (Delta ++ Delta')).
   apply IHHT2; permut_simpl.
@@ -338,7 +279,7 @@ assert (exists G0, exists G1, G' = G0 & Gamma ++ G1).
     rew_app; apply permut_trans with (l2:=G0); assumption.
 destruct H1 as [GH]; destruct H1 as [GT];
 subst G';
-apply t_letdia_get with (A:=A)(Gamma:=Gamma) (G:=GH ++ GT & (Delta ++ Delta')).
+apply t_letdia_get_LF with (A:=A)(Gamma:=Gamma) (G:=GH ++ GT & (Delta ++ Delta')).
 (* <*> A*)
 apply BackgroundSubsetImpl with (G:= (GH ++ GT & Gamma') & (Delta ++ Delta')).
   apply IHHT1;
@@ -364,7 +305,7 @@ apply BackgroundSubsetImpl with (G:=(((A :: nil) :: GH ++ GT & Gamma) & (Delta +
   exists nil; permut_simpl.
 permut_simpl.
 (* letdia_get 2 *)
-apply t_letdia_get with (A:=A)(G:=G) (Gamma:=Gamma).
+apply t_letdia_get_LF with (A:=A)(G:=G) (Gamma:=Gamma).
 apply IHHT1; permut_simpl.
 apply IHHT2; permut_simpl.
 assumption.
@@ -396,8 +337,8 @@ forall G M A
     permut G G' -> 
     forall Ctx, Mem Ctx G' -> Ctx = nil)
   (HT: G |= nil |- M ::: A),
-  value M \/ exists N, M |-> N.
-induction M; intros; eauto using value.
+  value_LF M \/ exists N, M |-> N.
+induction M; intros; eauto using value_LF.
 (* hyp *)
 inversion HT; destruct n; discriminate.
 (* appl *)
@@ -426,8 +367,8 @@ destruct H; eexists; constructor; eapply H.
 (* here *)
 inversion HT; subst.
 destruct (IHM A0 EmptyCtx HT0).
-left; apply val_here; assumption.
-right; destruct H; exists (here x); eauto using step.
+left; apply val_here_LF; assumption.
+right; destruct H; exists (here_LF x); eauto using step_LF.
 (* get_here *)
 inversion HT; subst.
 destruct (IHM A0 EmptyCtx).
@@ -441,14 +382,14 @@ apply BackgroundSubsetImpl with (G:=G0 & nil).
 assumption.
 exists nil; permut_simpl; assumption.
 left; econstructor; eassumption.
-right; destruct H; exists (get_here x); eauto using step.
+right; destruct H; exists (get_here_LF x); eauto using step_LF.
 (* letdia *)
 right; inversion HT; subst.
 destruct (IHM1 (<*>A0) EmptyCtx HT1).
 inversion H; subst; inversion HT1; subst.
-  exists [M//0]M2; eauto using step.
-  exists [M//0]M2; eauto using step.
-destruct H; exists (letdia x M2); eauto using step.
+  exists [M//0]M2; eauto using step_LF.
+  exists [M//0]M2; eauto using step_LF.
+destruct H; exists (letdia_LF x M2); eauto using step_LF.
 (* letdia_get *)
 right; inversion HT; subst.
 destruct (IHM1 (<*>A0) EmptyCtx).
@@ -462,63 +403,55 @@ apply BackgroundSubsetImpl with (G:=G0 & nil).
 assumption.
 exists nil; permut_simpl; assumption.
 inversion H; subst; inversion HT1; subst.
-  exists [M//0]M2; eauto using step.
-  exists [M//0]M2; eauto using step.
-destruct H; exists (letdia_get x M2); eauto using step.
+  exists [M//0]M2; eauto using step_LF.
+  exists [M//0]M2; eauto using step_LF.
+destruct H; exists (letdia_get_LF x M2); eauto using step_LF.
 Qed.
 
 (* Original formulations of modified typing rules can be reconstructed *)
 Lemma test_box:
   forall G G' Gamma M A,
     G & Gamma ++ G' |=  nil |- M ::: A ->
-      G ++ G' |= Gamma |- box M ::: [*]A.
-intros.
-constructor.
-apply BackgroundSubsetImpl with (G:=G & Gamma ++ G').
-assumption.
-exists nil; permut_simpl.
+      G ++ G' |= Gamma |- box_LF M ::: [*]A.
+intros; constructor;
+apply BackgroundSubsetImpl with (G:=G & Gamma ++ G');
+[ assumption | exists nil; permut_simpl].
 Qed.
 
 Lemma test_unbox_fetch:
   forall G G' Gamma Gamma' M A,
     G & Gamma ++ G' |= Gamma' |- M ::: [*] A ->
-      G & Gamma' ++ G' |= Gamma |- unbox_fetch M ::: A.
-intros.
-apply t_unbox_fetch with (G:=G ++ G') (Gamma:=Gamma').
-apply BackgroundSubsetImpl with (G:=G & Gamma ++ G').
-assumption.
-exists nil; permut_simpl.
-permut_simpl.
+      G & Gamma' ++ G' |= Gamma |- unbox_fetch_LF M ::: A.
+intros;
+apply t_unbox_fetch_LF with (G:=G ++ G') (Gamma:=Gamma');
+[apply BackgroundSubsetImpl with (G:=G & Gamma ++ G') | permut_simpl];
+[ assumption | exists nil; permut_simpl].
 Qed.
 
 Lemma test_get_here:
   forall G G' Gamma Gamma' M A,
     G & Gamma' ++ G' |= Gamma |- M ::: A ->
-      G & Gamma ++ G' |= Gamma' |- get_here M ::: <*> A.
-intros.
-apply t_get_here with (G:=G ++ G') (Gamma:=Gamma).
-apply BackgroundSubsetImpl with (G:=G & Gamma' ++ G').
-assumption.
-exists nil; permut_simpl.
-permut_simpl.
+      G & Gamma ++ G' |= Gamma' |- get_here_LF M ::: <*> A.
+intros;
+apply t_get_here_LF with (G:=G ++ G') (Gamma:=Gamma);
+[apply BackgroundSubsetImpl with (G:=G & Gamma' ++ G') | permut_simpl];
+[assumption | exists nil; permut_simpl].
 Qed.
 
 Lemma test_letdia_get:
   forall G G' Gamma Gamma' M N A B,
     G & Gamma' ++ G' |= Gamma |- M ::: <*>A ->
     (A::nil) :: G & Gamma ++ G' |= Gamma' |- N ::: B ->
-      G & Gamma ++ G' |= Gamma' |-  letdia_get M N ::: B.
-intros.
-apply t_letdia_get with (A:=A) (Gamma:=Gamma) (G:=G ++ G').
-apply BackgroundSubsetImpl with (G:=G & Gamma' ++ G').
-  assumption.
-  exists nil; permut_simpl.
-apply BackgroundSubsetImpl with (G:=(A::nil) :: G & Gamma ++ G').
-  assumption.  
-  exists nil; permut_simpl.
-permut_simpl.
+      G & Gamma ++ G' |= Gamma' |-  letdia_get_LF M N ::: B.
+intros;
+apply t_letdia_get_LF with (A:=A) (Gamma:=Gamma) (G:=G ++ G');
+[ apply BackgroundSubsetImpl with (G:=G & Gamma' ++ G') |
+  apply BackgroundSubsetImpl with (G:=(A::nil) :: G & Gamma ++ G') |
+  permut_simpl];
+  [assumption | exists nil; permut_simpl |
+   assumption | exists nil; permut_simpl ].
 Qed.
 
 End Lemmas.
 
-Close Scope is5_scope.
+Close Scope label_free_is5_scope.
