label-free/Substitution.v
@@ -1,24 +1,25 @@
 Require Export Syntax.
 Require Import Arith.
 Require Import List.
-Open Scope is5_scope.
+
+Open Scope label_free_is5_scope.
 
 Reserved Notation " [ M // x ] N " (at level 5).
 
-Fixpoint subst (M:te) (n:nat) (N:te) : te :=
+Fixpoint subst_LF (M:te_LF) (n:nat) (N:te_LF) : te_LF :=
 match N with
-| hyp n' => if (eq_nat_dec n n') then M else N
-| lam A N' => lam A ([M // S n]N')
-| appl N1 N2 => appl ([M//n]N1) ([M//n]N2)
-| box N' => box [M//n]N'
-| unbox N' => unbox [M//n]N'
-| unbox_fetch N'=> unbox_fetch [M//n]N'
-| here N' => here [M//n]N'
-| get_here N' => get_here [M//n]N'
-| letdia N1 N2 => letdia [M//n]N1 [M//S n]N2
-| letdia_get N1 N2 => letdia_get [M//n]N1 [M//S n]N2
+| hyp_LF n' => if (eq_nat_dec n n') then M else N
+| lam_LF A N' => lam_LF A ([M // S n]N')
+| appl_LF N1 N2 => appl_LF ([M//n]N1) ([M//n]N2)
+| box_LF N' => box_LF [M//n]N'
+| unbox_LF N' => unbox_LF [M//n]N'
+| unbox_fetch_LF N'=> unbox_fetch_LF [M//n]N'
+| here_LF N' => here_LF [M//n]N'
+| get_here_LF N' => get_here_LF [M//n]N'
+| letdia_LF N1 N2 => letdia_LF [M//n]N1 [M//S n]N2
+| letdia_get_LF N1 N2 => letdia_get_LF [M//n]N1 [M//S n]N2
 end
-where " [ M // x ] N " := (subst M x N) : is5_scope.
+where " [ M // x ] N " := (subst_LF M x N) : label_free_is5_scope.
 
 (* Substitute L[0] for n, L[1] for n+1,.. in M *)
 Fixpoint subst_list L n N :=
@@ -27,5 +28,4 @@ match L with
 | M :: L' => [M//n] (subst_list L' (S n) N)
 end.
 
-
-Close Scope is5_scope.
+Close Scope label_free_is5_scope.
