label-free/Syntax.v
@@ -1,30 +1,29 @@
 (* Types are exactly the same and should be shared between two languages *)
-Inductive ty :=
-| tvar: ty
-| tarrow: ty -> ty -> ty
-| tbox: ty -> ty
-| tdia: ty -> ty
+Inductive ty_LF :=
+| tvar_LF: ty_LF
+| tarrow_LF: ty_LF -> ty_LF -> ty_LF
+| tbox_LF: ty_LF -> ty_LF
+| tdia_LF: ty_LF -> ty_LF
 .
 
 (* So are notations *)
-Notation " A '--->' B " := (tarrow A B) (at level 30, right associativity) : is5_scope.
-Notation " '[*]' A " := (tbox A) (at level 30) : is5_scope.
-Notation " '<*>' A " := (tdia A) (at level 30) : is5_scope.
+Notation " A '--->' B " := (tarrow_LF A B) (at level 30, right associativity) : label_free_is5_scope.
+Notation " '[*]' A " := (tbox_LF A) (at level 30) : label_free_is5_scope.
+Notation " '<*>' A " := (tdia_LF A) (at level 30) : label_free_is5_scope.
 
-(* TODO: we'll need separate scopes for labeled and label-free version *)
-Open Scope is5_scope.
+Open Scope label_free_is5_scope.
 
-Inductive te :=
-| hyp: nat -> te
-| lam: ty -> te -> te
-| appl: te -> te -> te
-| box: te -> te
-| unbox: te -> te
-| unbox_fetch: te -> te
-| here: te -> te
-| get_here: te -> te
-| letdia: te -> te -> te
-| letdia_get: te -> te -> te
+Inductive te_LF :=
+| hyp_LF: nat -> te_LF
+| lam_LF: ty_LF -> te_LF -> te_LF
+| appl_LF: te_LF -> te_LF -> te_LF
+| box_LF: te_LF -> te_LF
+| unbox_LF: te_LF -> te_LF
+| unbox_fetch_LF: te_LF -> te_LF
+| here_LF: te_LF -> te_LF
+| get_here_LF: te_LF -> te_LF
+| letdia_LF: te_LF -> te_LF -> te_LF
+| letdia_get_LF: te_LF -> te_LF -> te_LF
 .
 
-Close Scope is5_scope.
+Close Scope label_free_is5_scope.
